\documentclass{article}
\usepackage{../cs170}
\AtBeginDocument{\RenewCommandCopy\qty\SI}

\def\title{HW 03}

\begin{document}

\maketitle

\question{}

\begin{center}
    \begin{circuitikz}
        \draw (0, 0) to[sV, l=\(V_s(t)\)] (0, 2) to[R, l=\(R\), a=\qty{10}{\ohm}] (2, 2) to[L, l=\(L\), a=\qty{1}{\micro\henry}] (4, 2) to[C, l=\(C\), a=\qty{1}{\nano\farad}] (6, 2) to[R, l=\(R_L\), a=\qty{1}{\kilo\ohm}] (6, 0) to[short] (0, 0) node[ground]{};
        \draw (6, 2) to[short] (7, 2) node[ocirc]{};
    \end{circuitikz}
\end{center}
The transfer function is
\begin{equation}
    H(s) = \frac{R_L}{R_L + R + sL + \frac{1}{sC}} = \frac{sR_L C}{1 + sC(R_L + R) + s^2 LC} = \frac{s \frac{R_L}{L}}{\frac{1}{LC} + s \frac{R_L + R}{L} + s^2} = K \frac{s \frac{\omega_0}{Q'}}{
    \omega_0^2 + s \frac{\omega_0}{Q'} + s^2}
\end{equation}
where \(\omega_0 = \frac{1}{\sqrt{LC}}\), \(Q' = \frac{1}{R_L + R} \sqrt{\frac{L}{C}}\), and \(K = \frac{R_L}{R_L + R}\).
At \(s = j\omega_0\), we have
\begin{equation}
    H(j\omega_0) = \frac{R_L}{R_L + R} \frac{\cancel{j \omega_0 \frac{\omega_0}{Q'}}}{\cancel{\omega_0^2} + \cancel{j \omega \frac{\omega_0}{Q'}} - \cancel{\omega_0^2}} = \frac{R_L}{R_L + R}
\end{equation}
\begin{center}
    \resizebox{0.8\textwidth}{!}{\input{q1.pgf}}
\end{center}
This is a variant of a band-pass filter.

\question{}

\begin{equation}
    H(s) = 50 \frac{s + 10000}{(s + 100) (s + 5000)}
\end{equation}
\begin{center}
    \resizebox{0.8\textwidth}{!}{\input{q2.pgf}}
\end{center}

\question{}

\begin{center}
    \begin{circuitikz}
        \draw (0, 0) node[ground]{} to[V, l=\(V_s\), invert] (0, 2) to[R, l=\(R_w\)] (2, 2) to[short] (2, 4) to[R, l=\(R_w\)] (4, 4) to[short] (5, 4) node[ocirc]{\(V_{L0}\)};
        \draw (2, 2) to[short] (2, 0) to[R, l=\(R_w\)] (4, 0) to[short] (5, 0) node[ocirc]{\(V_{L1}\)};
        \draw (4, 0) to[I, l=\(I_{L1}\)] (4, -2) node[ground]{};
        \draw (4, 4) to[I, l=\(I_{L0}\)] (4, 2) node[ground]{};
    \end{circuitikz}
\end{center}

\begin{subparts}
    \item With \(I_{L0} = I_{L1} = \qty{0}{\ampere}\),
    \begin{center}
        \begin{circuitikz}
            \draw (0, 0) node[ground]{} to[V, l=\(V_s\), invert] (0, 2) node[circ]{\(u_1\)} to[R, l=\(R_w\)] (2, 2) node[circ]{\(u_2\)} to[short] (2, 4) to[R, l=\(R_w\)] (4, 4) to[short] (5, 4) node[ocirc]{\(V_{L0}\)};
            \draw (2, 2) to[short] (2, 0) to[R, l=\(R_w\)] (4, 0) to[short] (5, 0) node[ocirc]{\(V_{L1}\)};
        \end{circuitikz}
    \end{center}
    Since we end up with an open circuit, we have \(V_{L0} = V_{L1} = V_s\).
    \item With \(I_{L0} = Q \delta(t)\), \(I_{L1} = \qty{0}{\ampere}\),
    \begin{center}
        \begin{circuitikz}
            \draw (0, 0) node[ground]{} to[V, l=\(V_s\), invert] (0, 2) node[circ]{\(u_1\)} to[R, l=\(R_w\)] (2, 2) node[circ]{\(u_2\)} to[short] (2, 4) to[R, l=\(R_w\)] (4, 4) to[short] (5, 4) node[ocirc]{\(V_{L0}\)};
            \draw (2, 2) to[short] (2, 0) to[R, l=\(R_w\)] (4, 0) to[short] (5, 0) node[ocirc]{\(V_{L1}\)};
            \draw (4, 4) to[I, l=\(I_{L0}\), a=\(Q \delta(t)\)] (4, 2) node[ground]{};
        \end{circuitikz}
    \end{center}
    % \(V_{L1}\) is still an open circuit, so \(V_{L1} = V_s\).
    % By superposition, nulling \(I_{L0}\) gives us \(V_{L0} = V_s\).
    % Nulling out \(V_s\) gives us the loop equation \(V_{L0} = -2R_w Q \delta(t)\).
    % Therefore, we have \(V_{L0} = V_s - 2R_w Q \delta(t)\).
    Performing node voltage analysis, we get the equations
    \begin{align}
        \frac{V_s - u_2}{R_w} &= \frac{u_2 - V_{L0}}{R_w} \\
        \frac{u_2 - V_{L0}}{R_w} &= Q \delta(t) \\
        V_{L1} &= u_2 \\
        \implies V_{L1} &= V_s - R_w Q \delta(t) \\
        \implies V_{L0} &= V_s - 2 R_w Q \delta(t)
    \end{align}
    \item The circuit is now
    \begin{center}
        \begin{circuitikz}
            \draw (0, 0) node[ground]{} to[V, l=\(V_s\), invert] (0, 2) to[R, l=\(R_w\)] (2, 2) to[short] (2, 4) to[R, l=\(R_w\)] (4, 4) to[short] (6, 4) node[ocirc]{\(V_{L0}\)};
            \draw (2, 2) to[short] (2, 0) to[R, l=\(R_w\)] (4, 0) to[short] (6, 0) node[ocirc]{\(V_{L1}\)};
            \draw (4, 4) to[C, l_=\(C_0\)] (4, 2) node[ground]{};
            \draw (4, 0) to[C, l_=\(C_1\)] (4, -2) node[ground]{};
            \draw (5, 4) to[I, l=\(I_{L0}\)] (5, 2) node[ground]{};
        \end{circuitikz} \\
        \begin{circuitikz}
            \draw (0, 0) node[ground]{} to[V, l=\(V_s \delta(t)\), invert] (0, 2) to[generic, l=\(R_w\)] (2, 2) node[circ]{\(u_1\)} to[short] (2, 4) to[generic, l=\(R_w\)] (4, 4) to[short] (6, 4) node[ocirc]{\(V_{L0}\)};
            \draw (2, 2) to[short] (2, 0) to[generic, l=\(R_w\)] (4, 0) to[short] (6, 0) node[ocirc]{\(V_{L1}\)};
            \draw (4, 4) to[generic, l_=\(\frac{1}{sC}\)] (4, 2) node[ground]{};
            \draw (4, 0) to[generic, l_=\(\frac{1}{sC}\)] (4, -2) node[ground]{};
            \draw (5, 4) to[I, l=\(Q\)] (5, 2) node[ground]{};
        \end{circuitikz}
    \end{center}
    We can null \(V_s\) and add it in later by superposition.
    Performing node voltage analysis gives us the equations
    \begin{align}
        \frac{u_1}{\cancel{R_w}} + \frac{u_1 - V_{L1}}{\cancel{R_w}} + \frac{u_1 - V_{L0}}{\cancel{R_W}} &= 0 \\
        \frac{u_1 - V_{L1}}{R_w} &= \frac{V_{L1}}{\frac{1}{sC}} \\
        \frac{u_1 - V_{L0}}{R_w} &= \frac{V_{L0}}{\frac{1}{sC}} + Q \\
        \implies 3u_1 - V_{L1} - V_{L0} &= 0 \\
        u_1 = (1 + s R_w C) V_{L1} &\implies V_{L1} = \frac{u_1}{1 + s R_w C} \\
        u_1 = (1 + s R_w C) V_{L0} + R_w Q &\implies V_{L0} = \frac{u_1 - R_w Q}{1 + s R_w C} \\
        3u_1 - \frac{u_1 - R_w Q}{1 + s R_w C} - \frac{u_1 - R_w Q}{1 + s R_w C} &= 0 \\
        \implies u_1 \left(3 - \frac{2}{1 + s R_w C}\right) &= -\frac{R_w Q}{1 + s R_w C} \\
        u_1 \left(\frac{1 + s 3 R_w C}{\cancel{1 + s R_w C}}\right) &= -\frac{R_w Q}{\cancel{1 + s R_w C}} \\
        \implies u_1 = -\frac{R_w Q}{1 + s 3 R_w C}
    \end{align}
    Finding \(V_{L1}\),
    \begin{align}
        V_{L1} = \frac{-R_w Q}{(1 + s 3 R_w C) (1 + s R_w C)} &= \frac{A}{1 + s 3 R_w C} + \frac{B}{1 + s R_w C} \\
        \implies -R_w Q &= A (1 + s R_w C) + B (1 + s 3 R_w C) \\
        s = -\frac{1}{R_w C} \implies B &= \frac{1}{2} R_w Q \\
        s = -\frac{1}{3 R_w C} \implies A &= -\frac{3}{2} R_w Q \\
        \implies V_{L1} &= R_w Q \left(-\frac{3}{2} \frac{1}{1 + s 3 R_w C} + \frac{1}{2} \frac{1}{1 + s R_w C}\right) \\
        \overset{\mathcal{L}^{-1}}{\implies} V_{L1}(t) &= V_s + \frac{Q}{2C} (-e^{-\frac{t}{3 R_w C}} + e^{-\frac{t}{R_w C}}) u(t)
    \end{align}
    Finding \(V_{L0}\),
    \begin{align}
        V_{L0} &= V_{L1} - \frac{R_w Q}{1 + s R_w C} \\
        \implies V_{L0}(t) &= V_s - \frac{Q}{2C} (e^{-\frac{t}{3 R_w C}} + e^{-\frac{t}{R_w C}}) u(t)
    \end{align}
\end{subparts}

\end{document}
